Started integrating the swap implementation into the quicksort implementation

boogie/perm_experimentation.bpl
@@ -24,6 +24,17 @@ function perm_of(a, b, perm: [int]int): bool
   (forall i: int :: vi(i) ==> a[i] == b[perm[i]])
 }
 
+// Returns true iff the elements of 'arr' are small (i.e. values in the range -3N to +3N)
+function has_small_elements(arr: [int]int): bool
+{
+  (forall i: int :: (0 <= i && i < N) ==> (-3 * N <= arr[i] && arr[i] <= 3 * N))
+}
+
+function sorted(a: [int]int, lo, up: int): bool
+{
+  (forall i, j: int :: lo <= i && i <= j && j <= up ==> a[i] <= a[j])
+}
+
 procedure init()
   modifies a, perm;
   ensures perm_of(a, old_a, perm);
@@ -45,6 +56,7 @@ procedure swap(i, j: int)
   ensures a[i] == old(a)[j];
   ensures a[j] == old(a)[i];
   ensures perm_of(a, old_a, perm);
+  ensures (forall k: int :: k != i && k != j ==> a[k] == old(a)[k]);
 {
   var temp: int;
   
@@ -57,15 +69,131 @@ procedure swap(i, j: int)
   a[j] := temp;
 }
 
-procedure sort()
+// Sorts 'a' using bucket sort or quick sort, as determined by has_small_elements(a)
+procedure sort() returns ()
   modifies a, perm;
   ensures perm_of(a, old_a, perm);
+  ensures sorted(a, 0, N - 1);
 {
   call init();
-  call swap(3, 4);
-  call swap(5, 6);
-  call swap(7, 1);
-  call swap(3, 6);
-  call swap(1, 4);
+  if (has_small_elements(a))
+  {
+    call bucketsort();
+  } else
+  {
+    call quicksort(0, N - 1);
+  }
 }
 
+procedure quicksort(lo, hi: int)
+  requires 0 <= lo;
+  requires lo <= hi;
+  requires hi < N;
+  requires perm_of(a, old_a, perm);
+  modifies a, perm;
+  ensures perm_of(a, old_a, perm);
+  ensures sorted(a, lo, hi);
+  ensures (forall k: int :: k < lo ==> a[k] == old(a)[k]);
+  ensures (forall k: int :: hi < k ==> a[k] == old(a)[k]);
+  ensures (forall k: int :: lo <= k && k <= hi ==> old(a)[lo - 1] <= old(a)[k])
+       ==> (forall k: int :: lo <= k && k <= hi ==> a[lo - 1] <= a[k]);
+  ensures (forall k: int :: lo <= k && k <= hi ==> old(a)[k] <= old(a)[hi + 1])
+       ==> (forall k: int :: lo <= k && k <= hi ==> a[k] <= a[hi + 1]);
+{
+  var p: int;
+   
+  if (lo == hi) {
+    return;
+  } else if (lo + 1 == hi) {
+    if (a[lo] > a[hi]) {
+      call swap(lo, hi);
+    }
+    return;
+  }
+  
+  call p := partition(lo, hi - 1, a[hi]);
+  
+  if (lo < p) {
+    call quicksort(lo, p - 1);
+  }
+  call quicksort(p, hi);
+  assert sorted(a, lo, p - 1);
+  assert sorted(a, p, hi);
+  //assert sorted(a, lo, hi);
+}
+
+procedure partition(lo, hi, pivot: int) returns (p: int)
+  requires 0 <= lo && lo <= hi && hi < N;
+  requires perm_of(a, old_a, perm);
+  modifies a, perm;
+  ensures perm_of(a, old_a, perm);
+  ensures lo <= p && p <= hi + 1;
+  ensures (forall k: int :: lo <= k && k < p ==> a[k] < pivot);
+  ensures (forall k: int :: p <= k && k <= lo ==> pivot <= a[k]);
+  ensures (forall k: int :: k < lo ==> a[k] == old(a)[k]);
+  ensures (forall k: int :: hi < k ==> a[k] == old(a)[k]);
+  ensures (forall k: int :: lo <= k && k <= hi ==> old(a)[lo - 1] <= old(a)[k])
+       ==> (forall k: int :: lo <= k && k <= hi ==> a[lo - 1] <= a[k]);
+  ensures (forall k: int :: lo <= k && k <= hi ==> old(a)[k] <= old(a)[hi + 1])
+       ==> (forall k: int :: lo <= k && k <= hi ==> a[k] <= a[hi + 1]);
+{
+  var i, j: int;
+  
+  i := lo;
+  j := hi;
+  
+  while (i < j)
+   invariant lo <= i && i <= j && j <= hi;
+   invariant perm_of(a, old_a, perm);
+   invariant (forall k: int :: lo <= k && k < i ==> a[k] < pivot);
+   invariant (forall k: int :: j < k && k <= hi ==> pivot <= a[k]);
+   invariant (forall k: int :: i < k && k < j ==> a[k] == old(a)[k]);
+   invariant (forall k: int :: k < lo ==> a[k] == old(a)[k]);
+   invariant (forall k: int :: hi < k ==> a[k] == old(a)[k]);
+   invariant (forall k: int :: lo <= k && k <= hi ==> old(a)[lo - 1] <= old(a)[k])
+       ==> (forall k: int :: lo <= k && k <= hi ==> a[lo - 1] <= a[k]);
+   invariant (forall k: int :: lo <= k && k <= hi ==> old(a)[k] <= old(a)[hi + 1])
+       ==> (forall k: int :: lo <= k && k <= hi ==> a[k] <= a[hi + 1]);
+  {
+    while (a[i] < pivot && i < j)
+      invariant lo <= i && i <= j && j <= hi;
+      invariant (forall k: int :: lo <= k && k < i ==> a[k] < pivot);
+    {
+      i := i + 1;
+    }
+    
+    if (i == j) {
+      break;
+    }
+    
+    while (pivot <= a[j] && i < j)
+      invariant lo <= i && i <= j && j <= hi;
+      invariant (forall k: int :: j < k && k <= hi ==> pivot <= a[k]);
+    {
+      j := j - 1;
+    }
+    
+    if (i == j) {
+      break;
+    }
+    
+    call swap(i, j);
+  }
+  
+  if (a[i] < pivot) {
+    i := i + 1;
+  }
+  
+  p := i;
+}
+
+
+procedure bucketsort()
+  requires perm_of(a, old_a, perm);
+  modifies a, perm;
+  ensures perm_of(a, old_a, perm);
+  ensures sorted(a, 0, N - 1);
+{
+  
+
+}
